lean/RubyCore/Proof/Judgment/ClsInv.lean
@@ -123,6 +123,9 @@ theorem KontOkJ.clsGrow {ans : Ty} {A : SemAxioms} :
       intro hg hch; exact .retValK hσ hms hsub (ih hg hch) hsu
   | casgnK hct hsct hrd hmods hsub _ hsu ih =>
       intro hg hch; exact .casgnK hct hsct hrd hmods hsub (ih hg hch) hsu
+  | casgnMK hicb himb hnbk hret hmeth hct hsct hrd hmods hsub _ hsu ih =>
+      intro hg hch
+      exact .casgnMK hicb himb hnbk hret hmeth hct hsct hrd hmods hsub (ih hg hch) hsu
   | hshKeyK hfv hmv hfp hmk hmvs hjv hpr hw _ hsu ih =>
       intro hg hch; exact .hshKeyK hfv hmv hfp hmk hmvs hjv hpr hw (ih hg hch) hsu
   | hshValK hfp hmk hmvs hpr hw _ hsu ih =>
